Started threading depth information

05TreeCode/TreeCode.thy
@@ -5,7 +5,7 @@ begin
 datatype tree_code = 
   TLookup nat
   | TPushCon nat
-  | TPushLam "tree_code list"
+  | TPushLam "tree_code list" nat
   | TApply
 
 datatype tclosure = 
@@ -20,7 +20,7 @@ inductive evalt :: "tree_code_state \<Rightarrow> tree_code_state \<Rightarrow> 
   evt_lookup [simp]: "lookup env x = Some v \<Longrightarrow> 
     TS vs ((env, TLookup x # cd) # sfs) \<leadsto>\<^sub>t TS (v # vs) ((env, cd) # sfs)"
 | evt_pushcon [simp]: "TS vs ((env, TPushCon k # cd) # sfs) \<leadsto>\<^sub>t TS (TConst k # vs) ((env, cd) # sfs)"
-| evt_pushlam [simp]: "TS vs ((env, TPushLam cd' # cd) # sfs) \<leadsto>\<^sub>t 
+| evt_pushlam [simp]: "TS vs ((env, TPushLam cd' (length env) # cd) # sfs) \<leadsto>\<^sub>t 
     TS (TLam env cd' # vs) ((env, cd) # sfs)"
 | evt_apply [simp]: "TS (v # TLam env' cd' # vs) ((env, TApply # cd) # sfs) \<leadsto>\<^sub>t 
     TS vs ((v # env', cd') # (env, cd) # sfs)"
@@ -38,7 +38,8 @@ next
 next
   case (evt_pushlam vs env cd' cd sfs)
   thus ?case 
-    by (induction "TS vs ((env, TPushLam cd' # cd) # sfs)" \<Sigma>'' rule: evalt.induct) simp_all 
+    by (induction "TS vs ((env, TPushLam cd' (length env) # cd) # sfs)" \<Sigma>'' rule: evalt.induct) 
+       simp_all 
 next
   case (evt_apply v env' cd' vs env cd sfs)
   thus ?case 
